theories/bucket.v
@@ -1,0 +1,241 @@
+From stdpp Require Import numbers list gmap.
+From listz Require Import listz.
+Notation len := length.
+From Stdlib Require Import Uint63.
+From Stdlib Require Import Array.PArray.
+From marble Require Import tactics bool int iteration loop wp logic array.
+
+(* This file contains the theory of "buckets", unboxed association lists. *)
+
+Hint Resolve not_elem_of_nil : marble.
+
+Ltac eq_decide v1 v2 := destruct (decide (v1 = v2)).
+
+Section Bucket.
+
+(* Type of keys *)
+Context {K : Type}.
+
+(* Type of values. *)
+Context {V : Type}.
+
+Parameter _eq : K -> K -> bool.
+
+Hint Rewrite
+  (@not_elem_of_cons (K * V)) : clist.
+
+(* The [_eq] function decides equality over keys. *)
+Declare Instance is_bool_eq :
+  ∀ k1 k2, isBool1 (_eq k1 k2) (k1 = k2).
+
+(* Although we could use a simple association list, we use the
+   following unboxed inductive data type for more efficient memory
+   usage *)
+Inductive bucket :=
+  | Nil : bucket
+  | Cons : K -> V -> bucket -> bucket.
+
+(* Isomorphism between buckets and lists. *)
+Fixpoint b2l b := match b with
+ |Nil => []
+ |Cons k v t => (k, v) :: b2l t
+ end.
+
+(* Proof that the [bucket] type is inhabited.  This is necessary for
+   total lookups on finite maps. *)
+Global Instance bucket_inh : Inhabited bucket :=
+  populate Nil.
+
+(* When reasoning over buckets, we use standard Rocq lists as opposed
+   to creating a separate theory over buckets. *)
+Definition assoc := list (K * V).
+
+(* Decidable equality over [K].  We use the [_eq] function to show
+   that equality is decidable. This instance is necessary for lookups
+   on finite maps. *)
+Instance dec_eq : EqDecision K.
+Proof.
+  intros x y.
+  pose is_bool_eq as H.
+  specialize H with x y.
+  unfold Decision.
+  unfold isBool1 in H.
+  destruct _eq; auto.
+Qed.
+
+Notation filter_key k l :=
+  (filter (fun (x : K * V) => eq x.1 k) l).
+
+(* -------------------------------------------------------------------------- *)
+
+(* Lemmas for filtering association lists *)
+
+Lemma filter_key_nin :
+  forall k b,
+    (∀ v : V, (k, v) ∉ b) ->
+    filter_key k b = [].
+Proof.
+  intros k b H1.
+  induction b as [|[k' v] t Ih]; auto.
+  rewrite filter_cons_False.
+  + apply Ih. intros v'.
+    specialize H1 with v'.
+    list in H1. by unpack.
+  + specialize H1 with v.
+    list in H1. unpack.
+    intros ?. by subst.
+Qed.
+
+Hint Rewrite
+  @filter_nil
+  @filter_cons_False
+  @filter_cons_True
+  using done : cfilter.
+
+Ltac filter := autorewrite with cfilter.
+
+Lemma filter_key_cons :
+  forall k k' v b1 b2,
+    filter_key k b1 = filter_key k b2 ->
+    filter_key k ((k', v)::b1) = filter_key k ((k', v) :: b2).
+Proof.
+  intros. eq_decide k k'; subst; filter; auto.
+  by f_equal.
+Qed.
+
+(* Association lists *)
+
+(* [(b', r) = remove_assoc k b] returns a new bucket [b'] where the
+first binding of key [k] is removed.  If there was no value associated
+with key [k], [r] is [false] and [b'] = [b], otherwise it is
+[true]. *)
+Fixpoint remove_assoc (k : K) (b : bucket) :=
+  match b with
+  |Nil => (false, Nil)
+  |Cons x v t =>
+     do b ← _eq x k;
+     if b then (true, t)
+     else
+       do (r, t) ← remove_assoc k t;
+       (r, Cons x v t)
+  end.
+
+(* [l' = remove_assoc_list k l] returns a list [l'] where the first
+   binding of key [k] is removed.
+   If no such binding exists then [l' = l]. *)
+Fixpoint remove_assoc_list (k : K) (l : list (K * V)) :=
+  match l with
+  |[] => []
+  |(k', v) :: t =>
+     if (decide (k = k'))
+     then t
+     else
+       (k', v) :: remove_assoc_list k t
+  end.
+
+(* If a binding is in the result of [remove_assoc_list], then it was
+in the original association list *)
+
+Lemma remove_assoc_in :
+  forall l k k' v,
+    (k', v) ∈ remove_assoc_list k l ->
+    (k', v) ∈ l.
+Proof.
+  intros l k k' v H1.
+  induction l as [|[k'' v'] t Ih]; simpl in H1.
+  - auto with marble.
+  - destruct decide; rewrite elem_of_cons; auto.
+    apply elem_of_cons in H1 as [H1 | H1]; auto.
+Qed.
+
+(* The list of bindings for [k] in [remove_assoc_list l] is equal to
+   [tl (filter_key k l)] *)
+
+Lemma remove_assoc_bucket_eq :
+  forall k b b',
+    b' = remove_assoc_list k b ->
+    filter_key k b' = tl (filter_key k b).
+Proof.
+  intros k b.
+  induction b as [|[k' v] t Ih]; simpl; intros b' H1; subst b'. auto.
+  case_decide.
+  - subst. by filter.
+  - filter. auto.
+Qed.
+
+(* The list of bindings for [k'] in [remove_assoc_list k b] is equal
+   to the list of bindings for [k'] in [l], provided that [k' ≠ k].*)
+
+Lemma remove_assoc_bucket_ne :
+  forall k k' b b',
+    b' = remove_assoc_list k b ->
+    k' ≠ k ->
+    filter_key k' b' = filter_key k' b.
+Proof.
+  intros k k' b.
+  induction b as [|[k'' v] t Ih]; simpl; intros b' H1 H2; subst b'; auto.
+  case_decide.
+  - subst. by filter.
+  - apply filter_key_cons. by apply Ih.
+Qed.
+
+Lemma remove_assoc_wp k b:
+  ∀ l, l = b2l b ->
+  wp (remove_assoc k b)
+    (λ r, let (r, b') := r in
+          ∃ l', l' = b2l b' ∧
+          isBool r (∃ v, (k, v) ∈ l) (∀ v, (k, v) ∉ l) ∧
+          l' = remove_assoc_list k l).
+Proof.
+  induction b as [|k' v b Ih]; simpl; intros; subst l.
+  - (* When the list is empty. *)
+    wp_ret. simpl. eauto with marble.
+  - (* When the list is non-empty. *)
+    simpl. wp_bind_eq. wp_if.
+    + (* If the current binding is equal to [k]. *)
+      subst k'. wp_ret. simpl.
+      pack; eauto.
+      { try constructor. }
+      { by rewrite decide_True. }
+    + (* If the current binding is not equal to [k]*)
+      wp_op Ih. intros [r b'] [l' ?].
+      unpack. eexists. subst l'.
+      pack; try by filter.
+      { destruct r; simpl in *.
+        - unpack. eexists. by constructor.
+        - intros. list.
+          split; auto. intros I. by injection I. }
+      { rewrite decide_False by auto.
+        simpl. by f_equal. }
+Qed.
+
+Fixpoint find_assoc (k : K) (b : bucket) : option V :=
+  match b with
+  |Nil => None
+  |Cons k' v t =>
+     if _eq k k'
+     then Some v
+     else find_assoc k t
+  end.
+
+Lemma find_assoc_wp k b :
+  ∀ b', b' = (filter_key k (b2l b)) ->
+  wp (find_assoc k b)
+    (λ o, o = head (map snd b')).
+Proof.
+  intros. induction b as [|k' v t Ih].
+  - wp_ret.
+  - simpl. wp_if.
+    + wp_ret. subst. simpl. by filter.
+    + wp_op Ih; auto. subst. simpl. by filter.
+Qed.
+
+End Bucket.
+
+Hint Rewrite
+  @filter_nil
+  @filter_cons_False
+  @filter_cons_True
+  using done : cfilter.
+
+Ltac filter := autorewrite with cfilter.
