theories/hmap.v
@@ -1,0 +1,301 @@
+From stdpp Require Import numbers list gmap.
+From marble Require bucket.
+From listz Require Import listz.
+From marble Require Import tactics.
+Notation len := length.
+(* This file contains auxiliary lemmas to reason over the model of
+   hash tables, that is, finite maps of keys to lists of values. *)
+Section Hmap.
+
+Context {K V : Type}.
+
+(* We need to know that the type of [K] is countably infinite in order
+   to use the theory of finite maps from [stdpp]. *)
+Existing Instance bucket.dec_eq.
+Declare Instance count_K : Countable K.
+
+(* [gmap] is an implementation of finite maps using binary trees.  *)
+Notation hmap := (gmap K (list V)).
+
+(* Some definitions to facilitate working with functions as infinite
+   maps.
+
+   Remark: we leverage the fact that the Instance of the inhabited
+   type class for lists is the empty list.*)
+Lemma lookup_total_empty_list (m : hmap) k :
+    m !! k = None ->
+    m !!! k = [].
+Proof.
+  intros H. rewrite lookup_total_alt.
+  by rewrite H.
+Qed.
+
+Lemma lookup_total_non_empty_list :
+  forall (m : hmap) k x t,
+    m !!! k = x :: t ->
+    m !! k = Some(x :: t).
+Proof.
+  intros m k x t H.
+  rewrite lookup_total_alt in H.
+  destruct (m !! k); simpl in *; f_equal; done.
+Qed.
+
+Lemma lookup_total_Some :
+  ∀ (m : hmap) k,
+    m !! k ≠ None →
+    m !! k = Some (m !!! k).
+Proof.
+  intros.
+  remember (m !! k) as l.
+  destruct l as [l|]. 2: done.
+  by rewrite lookup_total_correct with (x:=l).
+Qed.
+
+Hint Rewrite
+  lookup_total_Some
+  lookup_total_empty_list
+  using done : cmap.
+
+Hint Rewrite
+  (fin_maps.lookup_total_insert_ne (M:=gmap K) (A:=list V))
+  (fin_maps.lookup_total_insert_eq (M:=gmap K) (A:=list V))
+  using done : cmap.
+
+Ltac hmap := autorewrite with cmap.
+
+Tactic Notation "hmap" "in" hyp(h) :=
+  autorewrite with cmap in h.
+
+Tactic Notation "hmap" "in" "*" :=
+  autorewrite with cmap in *.
+
+Definition add (m : hmap) (k : K) (v : V) := <[k:= v :: m !!! k]> m.
+
+Lemma add_lookup_eq :
+  forall m k v, add m k v !!! k = v :: m !!! k.
+Proof.
+  intros.
+  unfold add.
+  by hmap.
+Qed.
+
+Lemma add_lookup_neq :
+  forall m k k' v,
+    k ≠ k' →
+    add m k v !!! k' = m !!! k'.
+Proof.
+  intros.
+  unfold add.
+  by hmap.
+Qed.
+
+Definition rm (m : hmap) (k : K) :=
+  <[k:=tl (m !!! k)]> m.
+
+Definition rm_add (m : hmap) (k : K) (v : V) :=
+  add (rm m k) k v.
+
+Definition cardinality (h : hmap) :=
+  (map_fold (fun _ v acc => acc + len v) 0 h)%Z.
+
+Lemma cardinality_empty :
+  cardinality ∅ = 0%Z.
+Proof.
+  apply map_fold_empty.
+Qed.
+
+Lemma cardinality_insert_fresh :
+  forall m k l n,
+    cardinality m = n ->
+    m !! k = None ->
+    cardinality (<[k:=l]>m) = (len l + n)%Z.
+Proof.
+  intros.
+  subst n.
+  unfold cardinality.
+  rewrite map_fold_insert; tc.
+Qed.
+
+Lemma add_ge :
+  ∀ n m, n >= 0 -> m >= 0 -> n + m >= 0.
+Proof.
+  lia.
+Qed.
+
+Lemma cardinality_nonneg :
+  ∀ m, cardinality m >= 0.
+Proof.
+  intros.
+  induction m as [|k l] using map_first_key_ind.
+  - by rewrite cardinality_empty.
+  - erewrite cardinality_insert_fresh; eauto.
+    generalize (@length_nonneg V l). lia.
+Qed.
+
+Lemma cardinality_delete_present :
+  forall m k l n,
+    cardinality m = n ->
+    m !! k = Some l ->
+    (cardinality (delete k m) + len l)%Z = n.
+Proof.
+  intros. subst n. unfold cardinality.
+  rewrite map_fold_delete with (m:=m); tc.
+Qed.
+
+Lemma cardinality_delete_present_alt :
+  forall m k l n,
+    cardinality m = n ->
+    m !! k = Some l ->
+    cardinality (delete k m) = (n - len l)%Z.
+Proof.
+  intros. subst. unfold cardinality.
+  rewrite map_fold_delete with (m:=m) (R:=eq); tc. lia.
+Qed.
+
+Lemma cardinality_insert :
+  forall m k l n,
+    cardinality m = n ->
+    cardinality (<[k:=l]>m) = (n + len l - len (m !!! k))%Z.
+Proof.
+  intros m k l n H1.
+  destruct (decide (m !! k = None)).
+  - hmap. erewrite cardinality_insert_fresh by auto.
+    length. lia.
+  - rewrite <- insert_delete_eq.
+    rewrite cardinality_insert_fresh with (n:=(n - len (m !!! k))%Z). lia.
+    + erewrite <- cardinality_delete_present_alt; auto with lia.
+      by hmap.
+    + by rewrite lookup_delete_eq.
+Qed.
+
+Lemma cardinality_delete :
+  forall m n k,
+    cardinality m = n ->
+    cardinality (delete k m) = (n - len (m !!! k))%Z.
+Proof.
+  intros m n k H1.
+  remember (m !! k) as l eqn:E.
+  destruct l as [l|].
+  + erewrite cardinality_delete_present_alt; eauto.
+    rewrite <- E. f_equal. symmetry.
+    by apply lookup_total_correct.
+  + hmap. length. by rewrite delete_id.
+Qed.
+
+Ltac cinsert n := erewrite cardinality_insert by auto.
+
+Lemma cardinality_empty_lists :
+  forall m,
+    (∀ k, m !!! k = []) →
+    cardinality m = 0%Z.
+Proof.
+  intros m Hempty.
+  induction m as [|k v m Hnone Hfirst Ih] using map_first_key_ind. by hmap.
+  erewrite cardinality_insert.
+  - hmap. list. specialize Hempty with k.
+    rewrite fin_maps.lookup_total_insert_eq in Hempty.
+    subst. by list.
+  - apply Ih. intros k'.
+    specialize Hempty with k'.
+    rewrite fin_maps.lookup_total_insert in Hempty.
+    case_decide; auto.
+    subst. by hmap.
+Qed.
+
+Lemma cardinality_add :
+  forall m n k v,
+    cardinality m = n ->
+    cardinality (add m k v) = (n + 1)%Z.
+Proof.
+  intros.
+  unfold add.
+  cinsert n.
+  length. lia.
+Qed.
+
+Lemma cardinality_rm_empty :
+  forall m n k,
+    cardinality m = n ->
+    m !!! k = [] ->
+    cardinality (rm m k) = n%Z.
+Proof.
+  intros m n k H1 H2.
+  unfold rm.
+  cinsert n.
+  rewrite H2. by length.
+Qed.
+
+Lemma cardinality_rm :
+  forall m n k,
+    cardinality m = n ->
+    m !!! k <> [] ->
+    cardinality (rm m k) = (n - 1)%Z.
+Proof.
+  intros.
+  unfold rm.
+  cinsert n.
+  remember (m !!! k) as l eqn:E.
+  destruct l. done.
+  subst. by length.
+Qed.
+
+Lemma cardinality_rm_add_empty :
+  forall m n k v,
+    cardinality m = n ->
+    m !!! k = [] ->
+    cardinality (rm_add m k v) = (n + 1)%Z.
+Proof.
+  intros.
+  unfold rm_add.
+  erewrite cardinality_add by auto.
+  erewrite cardinality_rm_empty by auto.
+  lia.
+Qed.
+
+Lemma cardinality_rm_add :
+  forall m n k v,
+    cardinality m = n ->
+    m !!! k <> [] ->
+    cardinality (rm_add m k v) = n.
+Proof.
+  intros.
+  unfold rm_add.
+  erewrite cardinality_add by auto.
+  erewrite cardinality_rm by auto. lia.
+Qed.
+
+Hint Rewrite
+  cardinality_empty
+  cardinality_add
+  cardinality_rm
+  cardinality_rm_empty
+  cardinality_rm_add
+  cardinality_rm_add_empty
+  using done : card.
+
+Lemma cardinality_extensionality :
+  ∀ (m1 : hmap) m2,
+    (∀ k, m1 !!! k = m2 !!! k) →
+    cardinality m1 = cardinality m2.
+Proof.
+  induction m1 as [|k v m1 Hnone Hfirst Ih] using map_first_key_ind;
+    intros m2 HLookup.
+  - hmap. rewrite cardinality_empty.
+    rewrite cardinality_empty_lists; auto.
+    intros k. specialize HLookup with k.
+    by rewrite lookup_total_empty in HLookup.
+  - erewrite cardinality_insert by auto.
+    hmap. rewrite Ih with (delete k m2).
+    { erewrite cardinality_delete; auto.
+      specialize HLookup with k. hmap in HLookup.
+      subst v. by list. }
+    { intros k'.
+      destruct (decide (k = k')).
+      - subst. rewrite fin_maps.lookup_total_delete_eq.
+        by hmap.
+      - rewrite fin_maps.lookup_total_delete_ne by auto.
+       specialize HLookup with k'.
+       by hmap in HLookup. }
+Qed.
+
+End Hmap.
